vale/code/crypto/aes/OptPublic.fsti
@@ -2,4 +2,4 @@ module OptPublic
 
 open Types_s
 
-val hkeys_reqs_pub (hkeys:FStar.Seq.seq quad32) (h_LE:quad32) (v2:quad32) : Prop_s.prop0
+val hkeys_reqs_pub (hkeys:FStar.Seq.seq quad32) (h_LE:quad32) : Prop_s.prop0
